refactor to 3 place relation

Order/Lib.lean
@@ -5,3 +5,11 @@ class Reflexive (op : α → α → Prop) : Prop where
 /-- A reflexive relation -/
 class Transitive (op : α → α → Prop) : Prop where
   trans : {a b c : α} → op a b -> op b c -> op a c
+
+/-- An associatve 3-place operato -/
+class Associative (op : α → α -> α → Prop) : Prop where
+  assoc : {x y z xy xyz : α} → op x y xy -> op xy z xyz -> ∃ yz, op y z yz ∧ op x yz xyz
+
+/-- A commutative 3-place operator -/
+class Commutative (op : α → α -> α → Prop) : Prop where
+  comm : {a b c : α} → op a b c -> op b a c
